Finalized the inv_ack repo and completed the first version of the binary representation part

applications.v
@@ -1,274 +1,126 @@
 Require Import Omega.
 Require Import prelims.
-Require Import countdown_repeater.
+Require Import repeater.
+Require Import increasing_expanding.
 Require Import inverse.
+Require Import countdown.
 
 (*
-=============================================================================
-**************** SECTION 5: DIV, LOG AND HIGHER LEVELS **********************
-=============================================================================
+===================================================================================
+************** SECTION 4.1 INVERSE HYPEROPS, DIVISION, LOG AND LOG* ***************
+===================================================================================
  *)
 
-(* This section contains applications of countdown and repeater.
-   Obviously we will use repeater to implement Hyperoperations, Knuth's Up Arrows,
-   and Ackermann function.
-   We use countdown to implement their inverses. We will introduce an inverse tower
-   for the Hyperoperation and Knuth's Up Arrow (which is just the truncation of the 
-   Hyperoperations).
+(* We use countdown to implement an inverse tower for the Hyperoperation.
    Interestingly, the 2nd, 3rd and 4th levels of this tower corresponds to division,
    log base b and log* base b, which are not defined in the Coq standard library. Our
    approach to them using countdown offers enough versatility and flexibility to
    substantiate easy and direct proof for a vast range of facts about these functions.
-   Lastly, we slightly modify this tower to get the inverse tower for the Peter-Ackermann
-   function, which is used to compute the Inverse Ackermann function, which is not
-   only an interesting application of countdown, but also an important one since it
-   computes the inverse Ackermann function in linear time. *)
+*)
 
-(* ****** 5.2. HYPEROPS ********************************* *)
+(* ****** INVERSE-HYPEROP TOWER ********************************* *)
 
-Definition hyperop_init (a n : nat) : nat :=
-  match n with 0 => a | 1 => 0 | _ => 1 end.
-
-Fixpoint hyperop_original (a n b : nat) : nat :=
-  match n with
-  | 0    => 1 + b
-  | S n' => let fix hyperop' (b : nat) :=
-            match b with
-            | 0 => hyperop_init a n'
-            | S b' => hyperop_original a n' (hyperop' b') 
-            end
-            in hyperop' b
-  end.
-
-Fixpoint hyperop (a n b : nat) : nat :=
-  match n with
-  | 0 => 1 + b
-  | S n' => repeater_from (hyperop_init a n') (hyperop a n') b
-  end.
-
-Theorem hyperop_correct :
-  forall n a b, hyperop n a b = hyperop_original n a b.
-Proof.
-  intros a n. induction n; trivial.
-  induction b; trivial.
-  simpl in *. rewrite IHb. trivial.
-Qed.
-
-Theorem hyperop_recursion :
-  forall n a b,
-    hyperop a (S n) (S b) = hyperop a n (hyperop a (S n) b).
-Proof. trivial. Qed.
-
-Theorem hyperop_1 : forall a b, hyperop a 1 b = b + a.
-Proof. intro a. induction b; [|rewrite hyperop_recursion, IHb]; trivial. Qed.
-
-Theorem hyperop_2 : forall a b, hyperop a 2 b = b * a.
-Proof.
-  intros a b. induction b; trivial.
-  rewrite hyperop_recursion, IHb, hyperop_1. simpl; omega.
-Qed.
-
-Theorem hyperop_3 : forall a b, hyperop a 3 b = a ^ b.
-Proof.
-  intros a b. induction b; trivial.
-  rewrite hyperop_recursion, IHb, hyperop_2.
-  simpl. apply Nat.mul_comm.
-Qed.
-
-Theorem hyperop_n_1 : forall n a, 2 <= n -> hyperop a n 1 = a.
-Proof.
-  intros n a Hn. do 2 (destruct n; [omega|]).
-  clear Hn. induction n; trivial.
-Qed.
-
-(* ****** 5.2. KNUTH ARROWS ********************************* *)
-
-Fixpoint knuth_arrow n a b :=
-  match n with
-  | 0 => b * a
-  | S n' =>
-    let fix knuth_arrow_n b0 :=
-        match b0 with
-        | 0 => 1
-        | S b0' => knuth_arrow n' a (knuth_arrow_n b0')
-        end in knuth_arrow_n b
-  end.
-
-Theorem knuth_arrow_recursion : forall n a b,
-    knuth_arrow (S n) a (S b) = knuth_arrow n a (knuth_arrow (S n) a b).
-Proof. trivial. Qed.
-
-Theorem knuth_arrow_hyperop : forall n a b,
-    knuth_arrow n a b = hyperop a (S(S n)) b.
-Proof.
-  intros n a.
-  induction n.
-  1: intro b; rewrite hyperop_2; trivial. 
-  induction b; trivial.
-  rewrite knuth_arrow_recursion, hyperop_recursion, IHb.
-  apply IHn.
-Qed.
-
-(* ****** 5.3. ACKERMANN FUNCS ********************************* *)
-
-Fixpoint ackermann_original (n m : nat) : nat :=
-  match n with
-  | 0    => 1 + m
-  | S n' => let fix ackermann' (m : nat) : nat :=
-              match m with
-              | 0 => ackermann_original n' 1
-              | S m' => ackermann_original n' (ackermann' m')
-              end
-            in ackermann' m
-  end.
-
-Fixpoint ackermann n m :=
-  match n with
-  | 0 => S m
-  | S n' => repeater_from (ackermann n' 1) (ackermann n') m
-  end.
-
-Theorem ackermann_correct :
-  forall n b, ackermann n b = ackermann_original n b.
-Proof.
-  intros n. induction n; trivial.
-  induction b. apply IHn.
-  simpl in *. rewrite IHb. trivial.
-Qed.
-
-Theorem ackermann_initial :
-  forall m, ackermann (S m) 0 = ackermann m 1.
-Proof. trivial. Qed.
-
-Theorem ackermann_recursion :
-  forall m n, ackermann (S m) (S n) = ackermann m (ackermann (S m) n).
-Proof. trivial. Qed.
-
-Theorem ack_hyperop : forall m n,
-    3 + ackermann m n = hyperop 2 m (3 + n).
-Proof.
-  induction m; trivial.
-  induction n.
-  - replace (3 + 0) with 3 by omega.
-    rewrite hyperop_recursion, ackermann_initial, IHm.
-    replace (3 + 1) with 4 by trivial.
-    f_equal. clear IHm.
-    induction m; trivial.
-    rewrite hyperop_recursion, hyperop_n_1; [trivial | omega].
-  - rewrite ackermann_recursion, IHm.
-    replace (3 + S n) with (S (3 + n)) by trivial.
-    rewrite hyperop_recursion, IHn; trivial.
-Qed.
-
-(* ****** 5.4. INVERSE-HYPEROP TOWER ********************************* *)
-
-Fixpoint inv_hyperop n a b :=
+Fixpoint inv_hyperop a n b :=
   match n with
   | 0 => b - 1
   | S n' =>
-    countdown_to match n' with 0 => a | 1 => 0 | _ => 1 end (inv_hyperop n' a) b
+    countdown_to (hyperop_init a n') (inv_hyperop a n') b
   end.
 
+(* Handy results to transform goals in involving inv_hyperop *)
 Theorem inv_hyperop_recursion :
   forall n a,
-    inv_hyperop (S n) a =
-    countdown_to (match n with | 0 => a | 1 => 0 | _ => 1 end)
-                 (inv_hyperop n a).
+    inv_hyperop a (S n) =
+    countdown_to (hyperop_init a n)
+                 (inv_hyperop a n).
 Proof. trivial. Qed.
 
-Theorem inv_hyperop_0_countdownable :
-  forall a k, countdownable_to k (inv_hyperop 0 a).
+(* Several results about first few levels of inv_hyperop.
+   Used to prove correctness of division and log later on *)
+
+Theorem inv_hyperop_0_contract_strict :
+  forall a k, contract_strict_above k (inv_hyperop a 0).
 Proof.
   intro a. split; intro n; simpl; omega.
 Qed.
 
 Theorem inv_hyperop_1 :
-  forall a b, inv_hyperop 1 a b = b - a.
+  forall a b, inv_hyperop a 1 b = b - a.
 Proof.
   intros a b.
   rewrite inv_hyperop_recursion.
   remember (b - a) as m.
   generalize dependent b. induction m.
   - intros b Hb.
-    apply countdown_to_recursion.
-    apply inv_hyperop_0_countdownable. omega.
+    apply countdown_recursion.
+    apply inv_hyperop_0_contract_strict.
+    unfold hyperop_init. omega.
   - intros b Hb. remember (m + a) as n.
     rewrite <- (IHm n) by omega.
-    replace n with (inv_hyperop 0 a b) by (simpl; omega).
-    apply countdown_to_recursion.
-    apply inv_hyperop_0_countdownable. omega.
+    replace n with (inv_hyperop a 0 b) by (simpl; unfold hyperop_init; omega).
+    apply countdown_recursion.
+    apply inv_hyperop_0_contract_strict.
+    unfold hyperop_init. omega.
 Qed.
 
 Corollary inv_hyperop_1_repeat :
-  forall a k m, repeat (inv_hyperop 1 a) k m = m - k * a.
+  forall a k m, repeat (inv_hyperop a 1) k m = m - k * a.
 Proof.
   intros a k m. induction k; [simpl; omega|].
-  remember (inv_hyperop 1 a) as f. simpl.
+  remember (inv_hyperop a 1) as f. simpl.
   rewrite IHk, Heqf, inv_hyperop_1; omega.
 Qed.
 
+(* Main theorem of this section. Establish the correctness of
+   the inverse hyperoperations' definition in inv_hyperop *)
 Theorem inv_hyperop_correct :
-  forall a n,
-    2 <= a ->
-    countdownable_to (match n with | 0 => a | 1 => 0 | _ => 1 end) (inv_hyperop n a) /\
-    upp_inv_rel (inv_hyperop n a) (hyperop a n).
+  forall a n, 2 <= a -> upp_inv_rel (inv_hyperop a n) (hyperop a n).
 Proof.
   intros a n Ha.
-  induction n.
-  1: split; [apply inv_hyperop_0_countdownable | intros n N; simpl; omega].
-  destruct n.
-  { split.
-    - split; intro n; rewrite inv_hyperop_1; omega.
-    - intros n N. rewrite inv_hyperop_1, hyperop_1. omega.
+  assert (forall m, repeatable_from (hyperop_init a m) (hyperop a m)).
+  { induction m.
+    - rewrite repeatable_simpl; split; simpl;
+      try split; try intros u v; omega.
+    - destruct m; try destruct m.
+      1, 3: try replace (hyperop a (S (S (S m)))) with
+           (repeater_from (hyperop a (S (S m))) (hyperop_init a (S (S m)))) by trivial;
+           apply repeater_repeatable; simpl; try omega; assumption.
+      rewrite repeatable_simpl. split.
+      intros u v. repeat rewrite hyperop_2. intros.
+      apply (mult_lt_compat_r _ _ _ H). omega.
+      simpl. omega.
   }
-  rewrite inv_hyperop_recursion.
-  replace (hyperop a (S (S n))) with
-      (repeater_from (match n with | 0 => 0 | S _ => 1 end) (hyperop a (S n)))
-    by trivial.
-  destruct IHn as [IHn0 IHn1].
-  split; [|apply countdown_repeater_upp_inverse; trivial].
-  destruct n; [|apply countdown_countdownable; trivial; apply IHn0].
-  split.
-  - intro n. rewrite countdown_to_repeat by apply IHn0.
-    rewrite inv_hyperop_1_repeat. assert (1 <= a) by omega.
-    apply (mult_le_compat_l 1 a n) in H. omega.
-  - intros n Hn.
-    destruct n; [omega|]. destruct n; [omega|]. 
-    rewrite <- le_S_n_m.
-    rewrite countdown_to_repeat by apply IHn0.
-    rewrite inv_hyperop_1_repeat. apply (Nat.le_sub_le_add_l).
-    apply (Nat.le_trans _ ((S n) * 2) _); [omega|].
-    apply (mult_le_compat_l 2 a (S n)) in Ha. omega.
+  induction n.
+  - simpl. intros u v. omega.
+  - destruct (H n) as [_ Hn]. apply countdown_repeater_upp_inverse; assumption.
 Qed.
 
-Corollary inv_hyperop_upp_inverse :
-  forall a n, (2 <= a) -> upp_inv_rel (inv_hyperop a n) (hyperop a n).
-Proof. apply inv_hyperop_correct. Qed.
-
-
-(* ****** 5.5. DIVISION AND LOGARITHM ********************************* *)
+(* ****** DIVISION AND LOGARITHM ********************************* *)
 
 (* Computes ceiling of b / a *)
-Definition div a b := inv_hyperop 2 a b.
+Definition div a b := inv_hyperop a 2 b.
 
 Theorem div_correct : forall a b m,
     1 <= a -> div a b <= m <-> b <= m * a.
 Proof.
   intros a b m Ha.
-  destruct a ; [omega|]. 
+  destruct a; [omega|]. 
   unfold div.
   rewrite inv_hyperop_recursion.
-  rewrite countdown_to_repeat by (split; intro n; rewrite inv_hyperop_1; omega).
-  rewrite inv_hyperop_1_repeat. omega.
+  rewrite countdown_repeat by (split; intro n; rewrite inv_hyperop_1; omega).
+  rewrite inv_hyperop_1_repeat. unfold hyperop_init. omega.
 Qed.
 
 (* Computes ceiling of log_a(b) *)
-Definition log a b := inv_hyperop 3 a b.
+Definition log a b := inv_hyperop a 3 b.
 
 Theorem log_correct : forall a b m,
     2 <= a -> log a b <= m <-> b <= a ^ m.
 Proof.
   intros a b m Ha.
   unfold log. rewrite <- hyperop_3.
-  apply inv_hyperop_upp_inverse; trivial.
+  apply inv_hyperop_correct; trivial.
 Qed.
+
+(* Computes log*_a(b). Its correctness is established in inv_hyperop_correct *)
+Definition logstar a b := inv_hyperop a 4 b.
