inv_ack.v
@@ -1,15 +1,17 @@
 Require Import Omega.
 Require Import Program.Basics.
+Require Import Logic.FunctionalExtensionality.
 Require Import prelims.
-Require Import countdown_repeater.
+Require Import repeater.
+Require Import increasing_expanding.
 Require Import inverse.
+Require Import countdown.
 Require Import applications.
 
-
 (*
-=============================================================================
-**************** SECTION 6: INVERSE ACKERMANN FUNCTION **********************
-=============================================================================
+==========================================================================
+************** SECTION 4.2 THE INVERSE ACKERMANN FUNCTION ****************
+==========================================================================
  *)
 
 (* This section contains the most important application of countdown,
@@ -17,19 +19,26 @@ Require Import applications.
    We first define an inverse tower for the Ackermann hierarchy, then
    write a theorem proving its correctness
    Then we define a structurally terminating definition for the inverse
-   Ackermann function, and prove its correctness using the above theorem *)
+   Ackermann function, and prove its correctness using the above theorem
+   We state and prove the correctness of the improvement, which runs in linear time
+   At the end, we also sketch a naive approach to the inverse Ackermann function,
+   which uses brute force search, and a massive improvement over it, but still slower
+   than our main method for inv_ack, although we do not prove it at the moment
+*)
 
-(* *********** 6.1. INVERSE ACKERMANN HIERARCHY ******************* *)
+(* *********** INVERSE ACKERMANN HIERARCHY ******************* *)
 
-Fixpoint inv_ack_hier m x :=
+(* Definition *)
+Fixpoint alpha m x :=
   match m with
   | 0 => x - 1
-  | S m' => countdown_to 1 (inv_ack_hier m') (inv_ack_hier m' x)
+  | S m' => countdown_to 1 (alpha m') (alpha m' x)
   end.
 
-Theorem inv_ack_hier_correct :
-  forall m, countdownable_to 1 (inv_ack_hier m) /\
-            upp_inv_rel (inv_ack_hier m) (ackermann m).
+(* Definition *)
+Theorem alpha_correct :
+  forall m, contract_strict_above 1 (alpha m) /\
+            upp_inv_rel (alpha m) (ackermann m).
 Proof.
   induction m.
   { split.
@@ -37,8 +46,8 @@ Proof.
     - intros n x. simpl. omega. }
   destruct IHm as [IHm0 IHm1]. split.
   - simpl. split; intro n;
-             rewrite countdown_to_antirecursion by apply IHm0;
-             apply (countdown_countdownable 1 _ 1) in IHm0;
+             rewrite countdown_antirecursion by apply IHm0;
+             apply (countdown_contract_strict 1 _ 1) in IHm0;
              destruct IHm0 as [IHm00 IHm01]; trivial.
     + specialize (IHm00 n). omega.
     + specialize (IHm01 n). omega.
@@ -46,26 +55,190 @@ Proof.
     rewrite <- repeat_S_comm.
     apply (upp_inv_repeat (S n) _ _) in IHm1.
     rewrite <- (IHm1 1 x), repeat_S_comm.
-    apply countdown_to_repeat. apply IHm0.
+    apply countdown_repeat. apply IHm0.
 Qed.
 
 
-(* *********** 6.2. INVERSE ACKERMANN FUNCTION ******************** *)
+(* *********** INVERTABILITY OF ACKERMANN FUNCTION ************ *)
 
-Fixpoint inv_ack_worker (f : nat -> nat) (n thr bud : nat) : nat :=
+(* Repeatability *)
+Lemma ack_repeatable : forall i, repeatable_from 0 (ackermann i).
+Proof.
+  induction i; split; try split;
+  intro n; try intro m; simpl; try omega;
+  apply (repeatable_monotone 0 1 _) in IHi; try omega;
+  repeat rewrite repeater_from_repeat;
+  repeat rewrite <- repeat_S_comm;
+  repeat rewrite <- repeater_from_repeat;
+  apply (repeater_repeatable _ 0 _) in IHi; try omega;
+  destruct IHi as [IHi0 IHi1];
+  [intro; apply IHi0; omega | |];
+  apply (Nat.le_trans _ (S (S n)) _); try apply IHi1; omega.
+Qed.
+
+(* Ackermann at level 1. It is useful for 2 purposes:
+   (1) Compute alpha 1 below, which is used in hard-coding the second level
+   for linear runtime.
+   (2) Serves to prove base case for "ack_incr_by_lvl"  *)
+Lemma ack_1 : forall n, ackermann 1 n = (S (S n)).
+Proof.
+  induction n; [|rewrite ackermann_recursion; rewrite IHn]; trivial.
+Qed.
+
+(* Alpha at level 1. Used in hard-coding the second level for linear runtime *)
+Lemma alpha_1 : alpha 1 = (fun n => n - 2).
+Proof.
+  assert (upp_inv_rel (alpha 1) (ackermann 1)) as H by apply alpha_correct.
+  assert (upp_inv_rel (fun n => n - 2) (ackermann 1)) as H'.
+  { intros n m. rewrite ack_1. omega. }
+  rewrite upp_inv_unique in H by
+   (intros n m; repeat rewrite ack_1; omega).
+  rewrite upp_inv_unique in H' by
+   (intros n m; repeat rewrite ack_1; omega).
+  rewrite H'. apply H.
+Qed.
+
+(* Below two results asserts that the diagonal Ackermann function is increasing,
+   hence has a proper upper inverse. We need them because we need to compute the inverse
+   value for the inv_ack correctness proof later *)
+
+(* Strict Increasing With Level *)
+Lemma ack_incr_by_lvl :
+    forall n, increasing (fun i => ackermann i n).
+Proof.
+  intro n. rewrite incr_S. intro i. generalize dependent n.
+  induction i; intro n.
+  - rewrite ack_1. simpl. omega.
+  - remember (S i) as p. destruct n.
+    + simpl. apply ack_repeatable. omega.
+    + rewrite ackermann_recursion. apply ack_repeatable.
+      assert (Hi := IHi).
+      rewrite Heqp in IHi. specialize (IHi (S n)).
+      rewrite ackermann_recursion in IHi.
+      rewrite <- incr_twoways in IHi by apply ack_repeatable.
+      apply (Nat.lt_trans _ (ackermann (S i) n) _); trivial.
+      clear IHi. induction n.
+      * simpl. apply Hi.
+      * repeat rewrite ackermann_recursion.
+        apply (Nat.lt_trans _ (ackermann i (ackermann (S p) n)) _).
+        apply ack_repeatable; assumption.
+        apply Hi.
+Qed.
+
+(* Diagonal Strict Increasing *)
+Lemma diag_ack_incr : increasing (fun n => ackermann n n).
+Proof.
+  intros n m Hnm. apply (Nat.lt_trans _ (ackermann n m) _);
+  [apply ack_repeatable| apply ack_incr_by_lvl]; assumption.
+Qed.
+
+
+(* *********** INVERSE ACKERMANN FUNCTION ******************** *)
+
+Fixpoint inv_ack_worker (f : nat -> nat) (n k bud : nat) : nat :=
   match bud with
-  | 0 => 0
+  | 0      => k
   | S bud' =>
-    match (n - thr) with
-    | 0 => 0
+    match (n - k) with
+    | 0   => k
     | S _ =>
-      match (countdown_to 1 f) with
-        g => S (inv_ack_worker (compose g f) (g n) (S thr) bud') end
+      let g := (countdown_to 1 f) in
+      inv_ack_worker (compose g f) (g n) (S k) bud'
     end
   end.
 
+(* Original defintion, runtime O(n^2) *)
 Definition inv_ack n :=
-  match (inv_ack_hier 0) with f => inv_ack_worker f (f n) 0 n end.
+  match (alpha 0) with f => inv_ack_worker f (f n) 0 n end.
+
+(* Intermediate lemma about inv_ack_worker *)
+Lemma inv_ack_worker_intermediate :
+    forall i n b, (i < alpha i n) -> (i < b) ->
+        (inv_ack_worker (alpha 0) (alpha 0 n) 0 b
+         = inv_ack_worker (alpha (S i)) (alpha (S i) n) (S i) (b - (S i))).
+    induction i.
+    - simpl. intros n b Hn Hb. unfold inv_ack_worker.
+      destruct b; try omega.
+      remember ((n - 1) - 0) as m. destruct m; try omega.
+      replace (S b - 1) with b by omega. trivial.
+    - intros n b Hn Hb. rewrite IHi.
+      + remember (S i) as p.
+        replace (alpha (S p)) with
+        (compose (countdown_to 1 (alpha p)) (alpha p)) by trivial.
+        unfold inv_ack_worker.
+        remember (alpha p n - p) as m. destruct m; try omega.
+        remember (b - p) as c. destruct c; try omega.
+        replace (b - S p) with c by omega.
+        rewrite <- Heqm. trivial.
+      + rewrite <- not_le. destruct (alpha_correct i) as [_ Halphai].
+        rewrite (Halphai i n). intro.
+        assert (n <= ackermann (S i) (S i)).
+        { apply (Nat.le_trans _ (ackermann i i) _); trivial.
+          apply Nat.lt_le_incl. apply diag_ack_incr. omega. }
+        destruct (alpha_correct (S i)) as [_ HalphaSi].
+        rewrite <- (HalphaSi (S i) n) in H0. omega.
+      + omega.
+Qed.
+
+(* Proof that inv_ack is correct *)
+Theorem inv_ack_correct :
+  upp_inv_rel inv_ack (fun k => ackermann k k).
+Proof.
+  rewrite upp_inv_unique by apply diag_ack_incr.
+  assert (forall n N : nat,
+            upp_inv (fun k : nat => ackermann k k) N <= n
+            <-> alpha n N <= n) as H.
+  { intros n N.
+    rewrite (upp_inv_correct (fun k : nat => ackermann k k)
+           diag_ack_incr n N). destruct (alpha_correct n) as [_ Hm].
+    symmetry. apply Hm. }
+  apply functional_extensionality. intro n.
+  remember (upp_inv (fun k : nat => ackermann k k) n) as m.
+  unfold inv_ack. assert (H0 := H). destruct m.
+  - specialize (H 0 n). rewrite <- Heqm in H.
+    assert (n <= 1) as Hn. { simpl in H. omega. }
+    destruct n; simpl; trivial; destruct n; simpl; trivial; omega.
+  - specialize (H m n). rewrite <- Heqm in H.
+    assert (m < alpha m n) as Hn by omega.
+    assert (S m < n) as Hmn.
+    { destruct (alpha_correct m) as [_ Hm]. rewrite <- not_le in Hn.
+      rewrite (Hm m n) in Hn. rewrite <- not_le. intro.
+      assert (ackermann m m <= m) by omega.
+      destruct (ack_repeatable m) as [_ Hackm].
+      destruct Hackm as [_ Hackm]. specialize (Hackm m).
+      omega. }
+    rewrite (inv_ack_worker_intermediate m n n).
+    assert (alpha (S m) n - (S m) = 0).
+    { specialize (H0 (S m) n). rewrite <- Heqm in H0. omega. }
+    unfold inv_ack_worker.
+    remember (n - S m) as p. destruct p; try omega.
+    + rewrite H1. trivial.
+    + assumption.
+    + omega.
+Qed.
+
+(* ****** INVERSE ACKERMANN BY HARD-CODING SECOND LEVEL ************* *)
+
+(* Definition by hard-coding the second alpha level, runtime O(n) *)
+Definition inv_ack' n :=
+  match n with
+  | 0 | 1 => 0
+  | _     => match (fun x => x - 2) with f
+             => inv_ack_worker f (f n) 1 (n - 1) end
+  end.
+
+(* Correctness proof *)
+Theorem inv_ack'_correct : inv_ack' = inv_ack.
+Proof.
+  apply functional_extensionality. intro n.
+  unfold inv_ack. unfold inv_ack'.
+  destruct n; try destruct n; trivial.
+  rewrite (inv_ack_worker_intermediate 0 _ _) by (simpl; omega).
+  rewrite alpha_1. trivial.
+Qed.
+
+
+(* *********** NAIVE INVERSE ACKERMANN FUNCTION ******************** *)
 
 Fixpoint inv_ack_naive (n : nat) (ans : nat) (bud : nat) : nat :=
   match bud with
@@ -124,36 +297,3 @@ Fixpoint inv_ack_target (n : nat) (ans : nat) (bud : nat) : nat :=
   end.
 
 Definition inv_ack_target_outer n := inv_ack_target n 0 n.
-
-
-(* Compute inv_ack 7. *)
-(* Compute ackermann 2 2. *)
-(* Time Compute inv_ack 62. *)
-(* Time Compute inv_ack_naive_outer 65. *) (* too slow *)
-(* Time Compute inv_ack_target_outer 65. *)
-(* Time Compute inv_ack 1000. *)
-(* Time Compute inv_ack_target_outer 1000. *)
-
-(* *********** 6.3. TIME ANALYSIS ********************* *)
-
-Definition next_lvl f := compose (countdown_to 1 f) f.
-
-Fixpoint alpha i : nat -> nat :=
-match i with
-| 0 => (fun b => b - 2)
-| S i' => next_lvl (alpha i')
-end.
-
-Fixpoint compose_sum (t : nat -> nat) (f : nat -> nat) k n : nat :=
-match k with
-| 0 => t n
-| S k' => t n + compose_sum t f k' (f n)
-end.
-
-Fixpoint rtime i n : nat :=
-match i with
-| 0 => 1
-| S i' => compose_sum (rtime i') (alpha i') (countdown_to 1 (alpha i') n) n + (alpha i n)
-end.
-
-(* Compute rtime 2 13. *)
