inverse.v
@@ -1,82 +1,96 @@
 Require Import Omega.
+Require Import Program.Basics.
+Require Import Logic.FunctionalExtensionality.
 Require Import prelims.
-Require Import countdown_repeater.
+Require Import repeater.
+Require Import increasing_expanding.
 
 (*
-=============================================================================
-****************** SECTION 2: UPPER AND LOWER INVERSE RELATION **************
-=============================================================================
+===================================================================================
+**** SECTION 3.1 INCREASING FUNCTIONS, UPPER INVERSE AND EXPANSIONS (2)************
+===================================================================================
  *)
 
-(* This section is for upper (and lower, not yet complete) inverse relations
-   The upper inverse is much less painful to define and used in proofs
-   The lower inverse is hadrder because it does not always exists, thus
-   requires more attention to edge cases, which results in complicated proofs.
-   Also: (n - 2) is the upper inverse of (n + 2) but NOT the lower inverse *)
+(* In Section 3.1, we introduce the notion of "upper inverse" (upp_inv),
+   increasing functions and why we prefer to consider inverse of
+   increasing functions only.
+   We prove several use results about upper inverse and increasing functions
+   We introduce "expansions" and how they are connected to increasing functions
+   through repeater.
+   Increasing functions that are strict expansions serve as the target for us
+   to compute the upper inverse with "countdown" later on. *)
 
-(* ****** 2.1. UPPER AND LOWER INVERSES ***************** *)
+(* In this PART 2 file, we deal with upper inverse of increasing functions *)
+
+
+(* ****** UPPER INVERSE ****************** *)
 
 (* f is the upper inverse of F: f N is the smallest n such that F n >= N *)
 Definition upp_inv_rel (f F : nat -> nat) : Prop :=
-  forall n N, f N <= n <-> N <= F n.
+    forall n N, f N <= n <-> N <= F n.
 
-Lemma upp_inv_rel_fact: forall f F, upp_inv_rel f F ->
-  forall n, f (F n) = n.
+(* An increasing F has a recursively definable upper inverse
+   Under assumption F is increasing, the below definition will compute its upper inverse
+   Do not use it for not always increasing functions
+   This is sort of why we are only interested in inverses of increasing functions
+   Inverses of other functions on naturals are hard to define neatly and do not
+   behave nicely.
+   This computation implies the upper inverse exists, which is useful for
+   proofs about worker functions later on *)
+Fixpoint upp_inv (F : nat -> nat) (n : nat) : nat :=
+  match n with
+  | 0 => 0
+  | S n' => let m := upp_inv F n' in
+            if F m =? n' then S m else m
+  end.
+
+(* Proof that the above upper inverse definition is correct *)
+Theorem upp_inv_correct :
+    forall F, increasing F -> upp_inv_rel (upp_inv F) F.
 Proof.
-  intros.
-  assert (f (F n) <= n) by (now rewrite (H _ _)).
-  assert (F n <= F (f (F n))). {
-    rewrite <- (H _ _). trivial. }
-  assert (n <= f (F n) \/ n > f (F n)) by omega.
-  destruct H2. omega.
-  Admitted.
-
-(* f is the lower inverse of F: f N is the largest n such that F n <= N *)
-Definition low_inv_rel_from_a (a : nat) (f F : nat -> nat) : Prop :=
-  forall n N, n <= f N <-> F n <= max a N.
-
-
-(* ****** 2.2. PROPERTIES PRESERVED BY INVERSES **************** *)
-
-(* Actually this section contains some redundant properties that I
-  haven't used in any proof *)
-
-(* Expansions, the counterpart of contractions *)
-Definition expanding (F : nat -> nat) : Prop :=
-  forall n, n <= F n.
-
-Definition expand_strict_from (a : nat) (F : nat -> nat) : Prop :=
-  forall n, a <= n -> S n <= F n.
-
-(* If the upper inverse of "F" is a contraction, then "F" is an expansion *) 
-Lemma contract_upp_inv_expand :
-  forall a f F,
-    contract_strict_from (S a) f -> upp_inv_rel f F ->
-    expand_strict_from a F.
-Proof.
-  intros a f F Hf HfF n Han.
-  rewrite <- (HfF n _). rewrite le_S_n_m.
-  apply (Hf (S n)). rewrite <- le_S_n_m. apply Han.
+  intros F HF n N. generalize dependent n.
+  induction N; intro n.
+  - simpl. omega.
+  - assert (N <= F (upp_inv F N)) as HN by (apply IHN; omega).
+    simpl. remember (upp_inv F N) as m. remember (F m =? N) as b.
+    symmetry in Heqb. destruct b.
+    + rewrite Nat.eqb_eq in Heqb. rewrite <- Heqb.
+      apply incr_twoways. apply HF.
+    + rewrite Nat.eqb_neq in Heqb.
+      assert (N < F m) as HNm by omega.
+      split; rewrite IHN;
+      [rewrite <- IHN; rewrite not_lt; rewrite incr_twoways by apply HF | ];
+      omega.
 Qed.
 
-(* Basically, since "F" is an expansion, "F n >= 1 + n > 0" *)
-Lemma contract_upp_inv_positive :
-  forall n f F, contract_strict_from 1 f -> upp_inv_rel f F -> 0 < F n.
+(* Proof that upper inverse is unique *)
+Theorem upp_inv_unique :
+    forall f F, increasing F -> (upp_inv_rel f F <-> f = upp_inv F).
 Proof.
-  intros n f F Hf HfF.
-  apply (Nat.le_trans _ (S n) _); [omega|]. 
-  apply (contract_upp_inv_expand 0 f F); trivial. omega.
+  intros f F HF.
+  assert (upp_inv_rel (upp_inv F) F) as H by (apply upp_inv_correct; apply HF).
+  split; intro.
+  - apply functional_extensionality. intro N.
+    assert (f N <= upp_inv F N).
+    { rewrite (H0 _ N). rewrite <- (H _ N). trivial. }
+    assert (upp_inv F N <= f N).
+    { rewrite (H _ N). rewrite <- (H0 _ N). trivial. }
+    omega.
+  - rewrite H0. trivial.
 Qed.
 
-(* If the upper inverse of "F" is increasing, so is "F" *)
-Lemma contract_incr_upp_inv_incr :
-  forall f F,
-    contract_strict_from 1 f -> increasing f ->
-    upp_inv_rel f F -> increasing F.
+(* Composing F's inverse and F gives identity *)
+Theorem upp_inv_compose :
+    forall f F, increasing F -> upp_inv_rel f F -> compose f F = id.
 Proof.
-  intros f F Hf_sh Hf_in HfF. rewrite incr_S. intro.
-  rewrite <- (HfF (S n) _). apply (Nat.le_trans _ n _); [|omega].
-  rewrite (HfF n _). trivial.
+  intros f F HF HfF. apply functional_extensionality. intro n.
+  unfold id. unfold compose.
+  assert (f (F n) <= n) as H0.
+  { rewrite (HfF n (F n)). trivial. }
+  assert (n <= f (F n)) as H1.
+  { rewrite not_lt. rewrite (incr_twoways F (f (F n)) n HF).
+    rewrite <- not_lt. rewrite <- (HfF (f (F n)) (F n)). trivial. }
+  omega.
 Qed.
 
 (* Repeat preserves upper inverse relation *)
@@ -88,57 +102,4 @@ Proof.
   intros n N. rewrite repeat_S_comm. split.
   - intro. rewrite IHk in H. simpl. apply HfF. apply H.
   - simpl; rewrite <- HfF; rewrite IHk; trivial.
-Qed.
-
-(*
-Lemma contract_low_inv_positive :
-forall n f F, contract_strict_from 1 f -> low_inv_rel_from_a 1 f F
--> (1 <= n) -> (0 < F n).
-Proof.
-intros n f F Hf HfF.
-apply (Nat.le_trans _ (S n) _). { omega. }
-apply (contract_low_inv_expand 1 f F); trivial.
-omega.
-Qed.
-
-Lemma contract_low_inv_expand :
-forall a f F, contract_strict_from a f -> low_inv_rel_from_a a f F -> expand_strict_from a F.
-Proof.
-intros a f F Hf HfF n Han.
-rewrite le_lt_S.
-rewrite <- not_le.
-assert (max a n = n) as Hman by (apply Nat.max_r_iff; trivial).
-rewrite <- Hman.
-rewrite <- (HfF _ n).
-rewrite Hman.
-apply (Hf n) in Han.
-omega.
-Qed.
-
-Lemma contract_incr_low_inv_incr :
-forall f F, contracting f -> increasing f -> low_inv_rel f F -> increasing F.
-Proof.
-intros f F Hf_sh Hf_in HfF. rewrite incr_S. intro.
-rewrite <- (HfF n _). apply (Nat.le_trans _ (S n) _).
-- omega.
-- rewrite (HfF (S n) _). trivial.
-Qed.
- *)
-
-(* ****** 2.3. COUNTDOWN - REPEATER - INVERSE PRESERVATION **************** *)
-
-(* This theorem is important. It says that the countdown and repeater will
-   preserve the upper inverse relation on their respective results
-   This is needed to prove that the tower (n - 2), ceil(n/2), ceil(log_2(n)), ...
-   is the upper inverse of the tower (n + 2), 2n, 2^n, ...
-   However I haven't cleaned that part in the old code yet *)
-
-Theorem countdown_repeater_upp_inverse : forall a f F,
-    countdownable_to a f -> upp_inv_rel f F ->
-    upp_inv_rel (countdown_to a f) (repeater_from a F).
-Proof.
-  intros a f F Haf HfF n N.
-  rewrite repeater_from_repeat.
-  apply (upp_inv_repeat n _ _) in HfF.
-  rewrite <- (HfF a N). apply countdown_to_repeat. apply Haf.
 Qed.
