prelims.v
@@ -4,15 +4,15 @@ Require Import Setoid.
 
 (*
 =============================================================================
-****************** SECTION 0: PRELIMINARIES *********************************
+****************** SECTION 1: PRELIMINARIES *********************************
 =============================================================================
  *)
 
-(* This file contains everything not put in the paper but will be useful
-   for the Coq proofs later on *)
+(* This file contains recurrently useful results and definitions
+   that are used throughout the subsequent files *)
 
 
-(* ****** 0.1. USEFUL LEMMAS ABOUT NAT ********************** *)
+(* ****** USEFUL LEMMAS ABOUT NAT ********************** *)
 
 Lemma le_S_n_m : forall n m : nat, n <= m <-> S n <= S m.
   intros. omega. Qed.
@@ -26,18 +26,11 @@ Lemma not_le: forall n m : nat, ~ n <= m <-> m < n.
 Lemma le_lt_S: forall n m : nat, S n <= m <-> n < m.
   intros. omega. Qed.
 
-
-(* ****** 0.2. CONTRACTIONS *************** *)
-
-(* Definition of general contractions *)
-Definition contracting (f : nat -> nat) : Prop := forall n, f n <= n.
-
-(* Basically: a contraction is strict from "a" iff "f n < n" for all "n > a" *)
-Definition contract_strict_from (a : nat) (f : nat -> nat) : Prop :=
-  forall n, a <= n -> S (f n) <= n.
+Lemma lt_S_le: forall n m : nat, n <= m <-> n < S m.
+  intros. omega. Qed.
 
 
-(* ****** 0.3. REPEATED APPLICATION AND CONTRACTION ************ *)
+(* ****** REPEATED APPLICATION ************ *)
 
 Fixpoint repeat (f: nat -> nat) (rep n : nat) : nat :=
   match rep with
@@ -55,104 +48,3 @@ Qed.
 Theorem repeat_plus :
   forall f k l n, repeat f (k + l) n = repeat f k (repeat f l n).
 Proof. induction k; trivial. simpl; intros; rewrite IHk; trivial. Qed.
-
-(* repeat of contractions make the result smaller *)
-Lemma repeat_contract :
-  forall f n k l,
-    contracting f -> k <= l -> repeat f l n <= repeat f k n.
-Proof.
-  intros f n k l Hf Hkl. induction l; inversion Hkl; trivial.
-  apply IHl in H0.
-  apply (Nat.le_trans _ (repeat f l n) _); [apply Hf | apply H0].
-Qed.
-
-(* strict version *)
-Lemma repeat_contract_strict :
-  forall a f n k,
-    contracting f -> contract_strict_from (S a) f ->
-    S a <= repeat f k n -> (S k) + repeat f (S k) n <= n.
-Proof.
-  intros a f n k Hf Haf Han. induction k.
-  1: simpl in Han; simpl; apply Haf in Han; omega. 
-  apply (Nat.le_trans _ (S k + repeat f (S k) n) _).
-  - apply Haf in Han. simpl. simpl in Han. omega.
-  - assert (S a <= repeat f k n) as Han0.
-    { apply (Nat.le_trans _ (repeat f (S k) n) _); [apply Han|].
-      apply Haf in Han. simpl. apply Hf. }
-    apply IHk in Han0. omega.
-Qed.
-
-(* 
- * Cleaning up to replace "S a <= b" with "a < b".
- * The exact same proof works. 
- *)
-Lemma repeat_contract_strict' :
-  forall a f n k,
-    contracting f ->
-    contract_strict_from (S a) f ->
-    a < repeat f k n ->
-    k + repeat f (S k) n < n.
-Proof. apply repeat_contract_strict. Qed.
-(* 
- * I wonder if maybe we can replace it like this everywhere,
- * provided it doens't affect the computation.
- *)
-
-(* Basically the existence of the countdown value for strict contractions
-   It asserts there is a minimum "l" for which repeating "f" "l" times from "n"
-   will give a result less than or equal to "a"
-   This is important for the proof of correctness in "countdown_compute.v" *)
-Lemma repeat_contract_strict_threshold :
-  forall a f n,
-    contracting f -> contract_strict_from (S a) f -> S a <= n ->
-    exists l, (S l) <= n /\ repeat f (S l) n <= a < repeat f l n.
-Proof.
-  intros a f n Hf Haf Han.
-  remember (n - a) as m.
-  destruct m; [omega|].
-  assert (forall b, (a <= b) -> f (S b) <= b) as Ha.
-  { intros b Hab. rewrite le_S_n_m. apply Haf. omega. }
-  generalize dependent a.
-  induction m.
-  - intros. exists 0.
-    simpl. split; [|split];
-             [|replace n with (S a) by omega; apply Ha|]; omega.
-  - intros. destruct (IHm (S a)); try omega.
-    + intros p Hp. apply Haf. omega.
-    + intros b Hab. apply Ha. omega.
-    + destruct H as [H0 H1]. destruct H1 as [Hl Hr]. inversion Hl.
-      2: exists x; split; [apply H0 | omega].
-      exists (S x). simpl. rewrite H1. split.
-      2: split; [apply Ha|]; omega.
-      apply (Nat.le_trans _ (S x + (repeat f (S x) n)) _);
-                  [simpl; rewrite H1; omega|].
-      apply (repeat_contract_strict a f n x); auto. omega.
-Qed.
-
-(* ****** 0.4. INCREASING FUNCTIONS ****************** *)
-
-(* Usual definition of increasing functions *)
-Definition increasing (f : nat -> nat) : Prop :=
-  forall n m, n <= m -> f n <= f m.
-
-(* A shortened equivalence of the notion of increasing *)
-Lemma incr_S : forall f,
-    increasing f <-> forall n, f n <= f (S n).
-Proof.
-  intro f. split; [intros; apply H; omega|].
-  unfold increasing. intros.
-  generalize dependent n.
-  induction m; [intros; inversion H0; omega|]. 
-  intros. inversion H0; [omega|].
-  apply IHm in H2. apply (Nat.le_trans _ (f m) _).
-  trivial. apply H.
-Qed.
-
-(* Repeat preserves increasing-ness *)
-Lemma repeat_incr : forall k f,
-    increasing f -> increasing (repeat f k).
-Proof.
-  unfold increasing. intros k f Hf.
-  induction k; trivial.
-  intros; apply Hf; apply IHk; trivial.
-Qed.
