bin_countdown.v
@@ -1,0 +1,203 @@
+Require Import BinNat.
+Require Import Omega.
+Require Import Logic.FunctionalExtensionality.
+Require Import Program.Basics.
+Require Import micromega.Lia.
+Require Import Nnat.
+Require Import bin_prelims.
+
+Require countdown.
+
+Open Scope N_scope.
+
+(* ****** CONTRACTIONS ****************** *)
+
+Definition contracting (f : N -> N) : Prop :=
+  forall n, f n <= n.
+
+Definition bin_contract_strict_above (a : N) (f : N -> N) : Prop :=
+  (contracting f) /\ (forall n, a < n -> f n <= N.div2 n).
+
+(* TODO: CONVERT THIS TO BINARY
+(* Upper inverse of strict from a expansions contract above a *)
+Theorem upp_inv_expand_contract_strict :
+    forall a f F, expand_strict_from a F -> upp_inv_rel f F -> contract_strict_above a f.
+Proof.
+  intros a f F HF HfF. destruct HF as [HF HaF].
+  split.
+  - apply (upp_inv_expand_contract _ F); assumption.
+  - intro n. destruct n; [omega|]. repeat rewrite <- le_S_n_m.
+    rewrite (HfF n _). apply HaF.
+Qed.
+*)
+
+(* ****** PROPERTIES OF CONTRACTIONS ************ *)
+
+(* Correct counterpart of contractions on nat *)
+Lemma contract_Nnat : forall f,
+    contracting f <-> countdown.contracting (to_nat_func f).
+Proof.
+  intro f. unfold to_nat_func. split; intros H n.
+  - rewrite le_nat_N. rewrite N2Nat.id. apply H.
+  - specialize (H (N.to_nat n)). simpl in H. rewrite le_nat_N in H.
+    repeat rewrite N2Nat.id in H. apply H.
+Qed.
+
+(* strict binary contractions are strict contractions on nat *)
+Lemma bin_contract_strict_Nnat : forall a f,
+   bin_contract_strict_above a f -> countdown.contract_strict_above (N.to_nat a) (to_nat_func f).
+Proof.
+  intros a f [Hf Haf]. split.
+  - rewrite <- contract_Nnat. apply Hf.
+  - intros n. unfold to_nat_func. repeat rewrite le_nat_N.
+    repeat rewrite Nat2N.inj_succ. repeat rewrite N2Nat.id.
+    intro Han. rewrite N.le_succ_l. apply (N.le_lt_trans _ (N.div2 (N.of_nat n)) _).
+    + apply Haf. lia.
+    + apply div2_contr; lia.
+Qed.
+
+(* repeat of contractions make the result smaller *)
+Lemma repeat_contract :
+  forall f n k l,
+    contracting f -> (k <= l)%nat -> repeat f l n <= repeat f k n.
+Proof.
+  intros f n k l Hf Hkl.
+  induction l; inversion Hkl; [lia |lia |].
+  apply IHl in H0.
+  apply (N.le_trans _ (repeat f l n) _); [apply Hf | apply H0].
+Qed.
+
+(* strict version *)
+Lemma repeat_bin_contract_strict :
+  forall a f n k,
+    bin_contract_strict_above a f ->
+    a < repeat f k n -> ((S k) + nat_size (repeat f (S k) n) <= nat_size n)%nat.
+Proof.
+  intros a f n k [Hf Haf] Han. induction k.
+  - simpl in Han. apply div2_nat_size; [lia| apply Haf; trivial]. 
+  - apply (Nat.le_trans _ (S k + nat_size (repeat f (S k) n)) _).
+    + simpl. simpl in Han. assert (H := Han). apply Haf in H.
+      apply div2_nat_size in H; lia.
+    + assert (a < repeat f k n) as Han0.
+    { apply (N.lt_le_trans _ (repeat f (S k) n) _); [apply Han| apply Hf]. }
+    apply (IHk Han0).
+Qed.
+
+
+(* ****** COUNTDOWN *************************************)
+
+Fixpoint countdown_worker (f : N -> N) (a n : N) (b : nat) : N :=
+  match b with
+  | O    => 0
+  | S b' => if (n <=? a) then 0
+             else 1 + countdown_worker f a (f n) b'
+  end.
+
+Definition countdown (f : N -> N) (a n : N) : N
+  := countdown_worker f a n (nat_size n).
+
+
+Lemma bin_contract_strict_threshold : forall a f n,
+    bin_contract_strict_above a f -> exists (t : nat),
+    (repeat f t n <= a
+    /\ forall k, repeat f k n <= a -> (t <= k)%nat).
+Proof.
+  intros a f n Haf. destruct Haf as [Hf Haf].
+  remember (N.to_nat (n - a)) as m eqn: Hm.
+  symmetry in Hm. rewrite <- Nat2N.id in Hm.
+  apply N2Nat.inj in Hm. generalize dependent a.
+  induction m.
+  - exists 0%nat. simpl. split.
+    + rewrite <- N.sub_0_le. apply Hm.
+    + intros. omega.
+  - intros a Haf Hm. rewrite Nat2N.inj_succ in Hm.
+    destruct (IHm (N.succ a)) as [x [Hax Haxn]];
+    [intros; apply Haf; lia| lia| ].
+    apply N.le_lteq in Hax. rewrite N.lt_succ_r in Hax.
+    destruct Hax as [Hax | Hax]; [exists x| exists (S x)];
+    split; try assumption.
+    + intros k Hk. apply Haxn. lia.
+    + rewrite <- N.lt_succ_r. simpl. rewrite Hax.
+      apply (N.le_lt_trans _ (N.div2 (N.succ a)) _).
+      * apply Haf. lia.
+      * apply div2_contr; lia.
+    + intros k Hk. assert (repeat f k n <= N.succ a) as H by lia.
+      apply Haxn in H. destruct H; [lia| omega].
+Qed.
+
+
+Lemma countdown_base : forall f a n b,
+    n <= a -> countdown_worker f a n b = 0.
+Proof.
+  intros f a n b Han. destruct b; trivial.
+  rewrite <- N.leb_le in Han. simpl. rewrite Han. trivial.
+Qed.
+
+Lemma countdown_intermediate : forall f a n b i,
+    contracting f -> ((S i) <= b)%nat -> (a < repeat f i n)
+    -> countdown_worker f a n b =
+       N.of_nat (S i) + countdown_worker f a (repeat f (S i) n) (b - (S i)).
+Proof.
+  intros f a n b i Hf.
+  generalize dependent b. generalize dependent n.
+  induction i; intros n b Hib Han; rewrite <- N.leb_gt in Han.
+  - destruct b. inversion Hib. replace (S b - 1)%nat with b by omega.
+    unfold countdown_worker. simpl in Han. rewrite Han. trivial.
+  - rewrite IHi.
+    + replace (b - S i)%nat with (S (b - S(S i))) by omega.
+      unfold countdown_worker. rewrite Han.
+      replace (N.of_nat (S(S i))) with (N.of_nat (S i) + 1).
+      apply N.add_assoc. rewrite N.add_1_r.
+      repeat rewrite Nat2N.inj_succ. trivial.
+    + omega.
+    + rewrite N.leb_gt in Han.
+      apply (N.lt_le_trans _ (repeat f (S i) n) _).
+      apply Han. apply Hf.
+Qed.
+
+Theorem countdown_repeat : forall f a n m,
+    bin_contract_strict_above a f ->
+    countdown f a n <= m <-> repeat f (N.to_nat m) n <= a.
+Proof.
+  intros f a n m Hf. unfold countdown.
+  destruct (bin_contract_strict_threshold a f n Hf) as [t [Ht0 Ht1]].
+  destruct t.
+  - simpl in Ht0. rewrite (countdown_base _ _ _ _ Ht0).
+    split; intro; try lia. apply (N.le_trans _ (repeat f 0 n) _).
+    apply repeat_contract. apply Hf. omega. apply Ht0.
+  - assert (a < repeat f t n) as Ht.
+    { rewrite N.lt_nge. intro. apply Ht1 in H. omega. }
+    rewrite (countdown_intermediate _ _ _ _ t).
+    rewrite (countdown_base _ _ _ _ Ht0). rewrite N.add_0_r.
+    replace m with (N.of_nat (N.to_nat m)) at 1 by apply N2Nat.id.
+    unfold N.le at 1. rewrite <- Nat2N.inj_compare.
+    rewrite Nat.compare_le_iff.
+    split; intro.
+    + apply (N.le_trans _ (repeat f (S t) n) _).
+      apply repeat_contract. apply Hf. apply H. apply Ht0.
+    + apply (Ht1 _ H).
+    + apply Hf.
+    + apply (Nat.le_trans _ (S t + nat_size (repeat f (S t) n))%nat _).
+      omega. apply (repeat_bin_contract_strict a _ _ _ Hf Ht).
+    + apply Ht.
+Qed.
+
+(* This countdown definition is consistent with its nat counterpart for
+   strict binary contractions *)
+Theorem countdown_correct : forall f a,
+    bin_contract_strict_above a f ->
+     countdown f a = to_N_func (countdown.countdown_to (N.to_nat a) (to_nat_func f)).
+Proof.
+  intros f a Haf. apply functional_extensionality. intro n.
+  assert (countdown.contract_strict_above (N.to_nat a) (to_nat_func f))
+  as Haf0 by apply (bin_contract_strict_Nnat a f Haf).
+  unfold to_N_func. apply le_antisym.
+  - rewrite countdown_repeat by apply Haf. rewrite Nat2N.id.
+    rewrite le_N_nat. rewrite to_N_func_repeat. unfold to_N_func.
+    rewrite Nat2N.id. rewrite <- countdown.countdown_repeat; trivial.
+  - rewrite le_N_nat. rewrite Nat2N.id.
+    rewrite countdown.countdown_repeat by apply Haf0.
+    rewrite to_nat_func_repeat. rewrite <- N_nat_func_id.
+    unfold to_nat_func. rewrite N2Nat.id. rewrite <- le_N_nat.
+    rewrite <- countdown_repeat. lia. trivial.
+Qed.
