countdown.v
@@ -1,0 +1,288 @@
+Require Import Omega.
+Require Import prelims.
+Require Import repeater.
+Require Import increasing_expanding.
+Require Import inverse.
+
+(*
+===================================================================================
+**** SECTION 3.2 INCREASING FUNCTIONS, UPPER INVERSE AND EXPANSIONS (2)************
+===================================================================================
+ *)
+
+(* In Section 3.2, we explore how to compute inverse of a function's repeater
+   solely from its own inverse, without directly computing the repeater itself.
+   The first lemma addresses this.
+   We base the definition of "contractions" and "countdown" on this observation
+   We also give a computation for countdown and prove several useful results about
+   it. *)
+
+(* The inverse of (repeater_from a F) is the minimum number of applications
+   of (inverse F) to the input to get a result less than or equal to a.
+   This serves as motivation to contractions and countdown *)
+Lemma upp_inv_repeater : forall a f F f',
+    upp_inv_rel f F -> upp_inv_rel f' (repeater_from F a)
+    -> (forall n m, f' n <= m <-> repeat f m n <= a).
+Proof.
+  intros a f F f' HfF Hf'F n m.
+  rewrite (Hf'F m n). rewrite repeater_from_repeat.
+  symmetry. apply (upp_inv_repeat m f F HfF a n).
+Qed.
+
+(* ****** CONTRACTIONS ****************** *)
+
+(* Definition of non-strict contractions *)
+Definition contracting (f : nat -> nat) : Prop :=
+  forall n, f n <= n.
+
+(* Definition of strict expansion *)
+Definition contract_strict_above (a : nat) (f : nat -> nat) : Prop :=
+  contracting f /\ (forall n, S a <= n -> S (f n) <= n).
+
+(* Upper inverse of expansions are contractions *)
+Theorem upp_inv_expand_contract :
+    forall f F, expanding F -> upp_inv_rel f F -> contracting f.
+Proof.
+  intros f F HF HfF n. rewrite (HfF n n). apply HF.
+Qed.
+
+(* Upper inverse of strict from a expansions contract above a *)
+Theorem upp_inv_expand_contract_strict :
+    forall a f F, expand_strict_from a F -> upp_inv_rel f F -> contract_strict_above a f.
+Proof.
+  intros a f F HF HfF. destruct HF as [HF HaF].
+  split.
+  - apply (upp_inv_expand_contract _ F); assumption.
+  - intro n. destruct n; [omega|]. repeat rewrite <- le_S_n_m.
+    rewrite (HfF n _). apply HaF.
+Qed.
+
+(* ****** PROPERTIES OF CONTRACTIONS ************ *)
+
+(* repeat of contractions make the result smaller *)
+Lemma repeat_contract :
+  forall f n k l,
+    contracting f -> k <= l -> repeat f l n <= repeat f k n.
+Proof.
+  intros f n k l Hf Hkl. induction l; inversion Hkl; trivial.
+  apply IHl in H0.
+  apply (Nat.le_trans _ (repeat f l n) _); [apply Hf | apply H0].
+Qed.
+
+(* strict version *)
+Lemma repeat_contract_strict :
+  forall a f n k,
+    contract_strict_above a f ->
+    S a <= repeat f k n -> (S k) + repeat f (S k) n <= n.
+Proof.
+  intros a f n k Hf Han. destruct Hf as [Hf Haf]. induction k.
+  1: simpl in Han; simpl; apply Haf in Han; omega. 
+  apply (Nat.le_trans _ (S k + repeat f (S k) n) _).
+  - apply Haf in Han. simpl. simpl in Han. omega.
+  - assert (S a <= repeat f k n) as Han0.
+    { apply (Nat.le_trans _ (repeat f (S k) n) _); [apply Han|].
+      apply Haf in Han. simpl. apply Hf. }
+    apply IHk in Han0. omega.
+Qed.
+
+
+
+(* ****** COUNTDOWN *************************************)
+
+(* Basically, repeats "f" "k" times or until we go below "a".
+   Output "min(k, min{l : repeat f l n <= a})" *)
+Fixpoint countdown_worker (a : nat) (f : nat -> nat) (n k : nat) : nat :=
+  match k with
+  | 0    => 0
+  | S k' => match (n - a) with
+            | 0 => 0
+            | _ => S (countdown_worker a f (f n) k') end
+  end.
+
+(* Actual defintion. We give the worker a budget of "n" steps, which
+   guarantees it reach below "a" before terminating *)
+Definition countdown_to a f n := countdown_worker a f n n.
+
+
+(* *** COUNTDOWN CORRECTNESS THEOREMS *** *)
+
+(* INITIAL VALUE THEOREM
+   Basically countdown returns 0 if "n" is already below "a" *)
+Theorem countdown_init : forall a f n k,
+    n <= a -> countdown_worker a f n k = 0.
+Proof.
+  intros a f n k Hna.
+  unfold countdown_worker.
+  destruct k; trivial.
+  replace (n - a) with 0 by omega; trivial.
+Qed.
+
+
+(* EXISTENCE OF COUNTDOWN VALUE LEMMA *)
+(* Basically the existence of the countdown value for strict contractions
+   It asserts there is a minimum "l" for which repeating "f" "l" times from "n"
+   will give a result less than or equal to "a" *)
+Lemma repeat_contract_strict_threshold :
+  forall a f n,
+    contract_strict_above a f -> S a <= n ->
+    exists l, (S l) <= n /\ repeat f (S l) n <= a < repeat f l n.
+Proof.
+  intros a f n Hf Han. destruct Hf as [Hf Haf].
+  remember (n - a) as m.
+  destruct m; [omega|].
+  assert (forall b, (a <= b) -> f (S b) <= b) as Ha.
+  { intros b Hab. rewrite le_S_n_m. apply Haf. omega. }
+  generalize dependent a.
+  induction m.
+  - intros. exists 0.
+    simpl. split; [|split];
+             [|replace n with (S a) by omega; apply Ha|]; omega.
+  - intros. destruct (IHm (S a)); try omega.
+    + intros p Hp. apply Haf. omega.
+    + intros b Hab. apply Ha. omega.
+    + destruct H as [H0 H1]. destruct H1 as [Hl Hr]. inversion Hl.
+      2: exists x; split; [apply H0 | omega].
+      exists (S x). simpl. rewrite H1. split.
+      2: split; [apply Ha|]; omega.
+      apply (Nat.le_trans _ (S x + (repeat f (S x) n)) _);
+                  [simpl; rewrite H1; omega|].
+      apply (repeat_contract_strict a f n x). split; assumption. omega.
+Qed.
+
+
+(* INTERMEDIATE STATE LEMMA
+   Similar to the general recursion formula for "countdown_recurse_rel" *)
+Theorem countdown_intermediate : forall a f n k i,
+    contracting f -> S i <= k ->
+    S a <= repeat f i n ->
+    countdown_worker a f n k =
+    (S i) + countdown_worker a f (repeat f (S i) n) (k - (S i)).
+Proof.
+  assert (forall a f n k,
+             contracting f -> 1 <= k -> S a <= n ->
+             countdown_worker a f n k =
+             1 + countdown_worker a f (f n) (k - 1) ) as case_0.
+  { simpl. intros a f n k Hf Hk Ha.
+    destruct k; [omega|]. 
+    replace (S k - 1) with k by omega.
+    unfold countdown_worker.
+    replace (n - a) with (S (n - S a)) by omega. trivial.
+  }
+  intros a f n k i Hf Hik Hai.
+  induction i; [simpl; apply case_0; trivial|]. rewrite IHi; [|omega|].
+  - simpl. remember (f (repeat f i n)) as m.
+    remember (k - S i) as l.
+    replace (k - S(S i)) with (l - 1) by omega.
+    rewrite case_0; [omega | trivial | omega|].
+    simpl in Hai. rewrite Heqm. trivial.
+  - apply (Nat.le_trans _ (repeat f (S i) n) _); [trivial | apply Hf].
+Qed.
+
+(* COUNTDOWN VS REPEAT THEOREM
+   Correctness theorem for this countdown defintion *)
+Theorem countdown_repeat : forall a f n k,
+    contract_strict_above a f -> countdown_to a f n <= k <-> repeat f k n <= a.
+Proof.
+  intros a f n k Haf. inversion Haf as [Hf _].
+  unfold countdown_to; split.
+  - intro. rewrite not_lt. intro.
+    rewrite (countdown_intermediate a f n n k Hf) in H; [omega | trivial..].
+    apply (Nat.le_trans _ (S k + (repeat f (S k) n)) _); [omega|].
+    apply (repeat_contract_strict a f n k Haf H0). 
+  - intro. destruct k.
+    1: simpl in H; rewrite (countdown_init a f n); omega; apply H. 
+    remember (n - a) as m.
+    destruct m; [rewrite countdown_init; omega|]. 
+    destruct (repeat_contract_strict_threshold a f n Haf); [omega|].
+    destruct H0 as [Hx0 [Hxl Hxr]].
+    assert (countdown_worker a f n n = S x) as Hx.
+    { rewrite (countdown_intermediate a f n n x);
+        [|apply Hf | apply Hx0| apply Hxr].
+      rewrite countdown_init. omega. apply Hxl.
+    }
+    rewrite Hx. apply not_le. intro.
+    apply (repeat_contract f n (S k) x) in H0.
+    omega. apply Hf.
+Qed.
+
+(* RECURSION FOR CONTRACTORS THEOREM *)
+Theorem countdown_recursion : forall a f n,
+    contract_strict_above a f ->
+    (n <= a -> countdown_to a f n = 0) /\
+    (S a <= n -> countdown_to a f n = S (countdown_to a f (f n))).
+Proof.
+  intros a f n Hf. split.
+  1: intro Han; unfold countdown_to; apply countdown_init; apply Han.
+  intro Han.
+  assert (countdown_to a f n <= S (countdown_to a f (f n))) as G1.
+  { rewrite countdown_repeat by apply Hf.
+    rewrite repeat_S_comm.
+    rewrite <- countdown_repeat by apply Hf.
+    trivial. }
+  assert (1 <= countdown_to a f n) as G0.
+  { rewrite le_lt_S. rewrite <- not_le.
+    rewrite countdown_repeat by apply Hf.
+    simpl. omega. }
+  assert (countdown_to a f (f n) <= countdown_to a f n - 1).
+  { rewrite countdown_repeat by apply Hf.
+    rewrite <- repeat_S_comm.
+    replace (S (countdown_to a f n - 1)) with (countdown_to a f n) by omega.
+    rewrite <- countdown_repeat by apply Hf. trivial. }
+  omega.
+Qed.
+
+Corollary countdown_antirecursion : forall a f n,
+    contract_strict_above a f -> countdown_to a f (f n) = countdown_to a f n - 1.
+Proof.
+  intros a f n Haf.
+  assert (H := Haf).
+  destruct (Nat.lt_ge_cases a n) as [Han | Han];
+    apply (countdown_recursion a f n) in H.
+  1: apply H in Han; omega.
+  assert (f n <= a) as Hafn.
+  { apply (Nat.le_trans _ n _); [apply Haf | apply Han]. }
+    apply (countdown_recursion a f (f n)) in Haf.
+    apply Haf in Hafn. apply H in Han. omega.
+Qed.
+
+
+(* STRICT CONTRACTIVENESS PRESERVATION THEOREM *)
+Theorem countdown_contract_strict : forall a f t,
+    1 <= a -> contract_strict_above a f ->
+    contract_strict_above t (countdown_to a f).
+Proof.
+  intros a f t Ha Haf. split.
+  - intro n. rewrite countdown_repeat by apply Haf.
+    rewrite not_lt. intro.
+    apply repeat_contract_strict in H; [omega | apply Haf..].
+  - intros n Hn. destruct n; [omega|].
+    rewrite <- le_S_n_m.
+    rewrite countdown_repeat by apply Haf.
+    destruct n;  trivial.
+    remember (repeat f n (S (S n)) - a) as m. destruct m.
+    1: apply (Nat.le_trans _ (repeat f n (S (S n))) _); [apply Haf | omega]. 
+    assert (S n + repeat f (S n) (S (S n)) <= (S n) + a).
+    { apply (Nat.le_trans _ (S (S n)) _);
+      [apply (repeat_contract_strict a _ _ _ Haf)|]; omega.
+    }
+    omega.
+Qed.
+
+(* ****** COUNTDOWN - REPEATER - INVERSE PRESERVATION **************** *)
+
+(* This theorem is important. It says that the countdown and repeater will
+   preserve the upper inverse relation on their respective results
+   This is needed to prove the correctness of inverse hypeoperations and
+   inverse Ackermann towers built with countdown later on *)
+
+Theorem countdown_repeater_upp_inverse : forall a f F,
+    expand_strict_from a F -> upp_inv_rel f F ->
+    upp_inv_rel (countdown_to a f) (repeater_from F a).
+Proof.
+  intros a f F HaF HfF n N.
+  apply (upp_inv_expand_contract_strict a f F) in HaF.
+  rewrite repeater_from_repeat.
+  apply (upp_inv_repeat n _ _) in HfF.
+  rewrite <- (HfF a N). apply countdown_repeat.
+  1,2 : assumption.
+Qed.
