Makefile
@@ -1,33 +1,44 @@
 CC=COQC
-
 .PHONY: all
-all: prelims.vo countdown_repeater.vo \
-	inverse.vo applications.vo \
-	inv_ack.vo inv_ack_hier.vo
+all: prelims.vo repeater.vo increasing_expanding.vo  inverse.vo countdown.vo applications.vo inv_ack.vo bin_prelims.vo bin_repeater.vo bin_countdown.vo bin_inv_ack.vo
 
 prelims.vo: prelims.v
 	$(CC) prelims.v
 
-countdown_repeater.vo: prelims.vo countdown_repeater.v
-	$(CC) countdown_repeater.v
+repeater.vo: prelims.vo repeater.v
+	$(CC) repeater.v
 
-inverse.vo: prelims.vo countdown_repeater.vo inverse.v
+increasing_expanding.vo: repeater.vo increasing_expanding.v
+	$(CC) increasing_expanding.v
+
+inverse.vo: prelims.vo repeater.vo increasing_expanding.vo inverse.v
 	$(CC) inverse.v
 
-applications.vo: prelims.vo countdown_repeater.vo inverse.vo applications.v
-	$(CC) applications.v
+countdown.vo: prelims.vo repeater.vo increasing_expanding.vo inverse.vo countdown.v
+	$(CC) countdown.v
 
-inv_ack.vo: prelims.vo countdown_repeater.vo inverse.vo applications.vo inv_ack.v
+applications.vo: prelims.vo repeater.vo increasing_expanding.vo inverse.vo countdown.vo  applications.v
+	$(CC) applications.v
+	
+inv_ack.vo: prelims.vo repeater.vo increasing_expanding.vo inverse.vo countdown.vo  applications.vo inv_ack.v
 	$(CC) inv_ack.v
 
-inv_ack_hier.vo: inv_ack_hier.v
-	$(CC) inv_ack_hier.v
+bin_prelims.vo: prelims.vo bin_prelims.v
+	$(CC) bin_prelims.v
+
+bin_repeater.vo: repeater.vo bin_prelims.vo bin_repeater.v
+	$(CC) bin_repeater.v
+
+bin_countdown.vo: countdown.vo bin_prelims.vo bin_repeater.vo bin_countdown.v
+	$(CC) bin_countdown.v
+
+bin_inv_ack.vo: inv_ack.vo bin_prelims.vo bin_repeater.vo bin_countdown.vo bin_inv_ack.v
+	$(CC) bin_inv_ack.v
 
 .PHONY: paper
 paper:
 	cd paper; pdflatex inv-ack.tex; cd -
-
-
+	
 .PHONY: clean
 clean:
 	rm -f *.vo *.glob paper/inv-ack.pdf paper/*.aux paper/*.log paper/*.out paper/*.spl
